Lazy Eager on FinType

theories/crypto/rom/PROM.ec
@@ -764,3 +764,111 @@ qed.
 end section.
 
 end GenEager.
+
+abstract theory FinGenEager.
+
+clone include GenEager.
+
+clone FinType as FinFrom with
+  type t <- from.
+
+module FinRO : RO = {
+  include RO [set, rem]
+
+  proc init () = {
+    var l;
+    l <- FinFrom.enum;
+    RO.init();
+    while (l <> []) {
+      RO.sample(head witness l);
+      l <- behead l;
+    } 
+  }
+
+  proc get (x:from) = {
+    return oget RO.m.[x];
+  }
+  
+  proc sample(x : from) = { 
+  }
+
+}.
+
+module MainD (D:RO_Distinguisher, RO:RO) = {
+  proc distinguish(x:input) = {
+    var b;
+    RO.init();
+    b <@ D(RO).distinguish(x);
+    return b;
+  }
+}.
+
+module type FinRO_Distinguisher(G : RO) = {
+  proc distinguish(_:input): output { G.init G.get G.set G.sample }
+}.
+
+section PROOFS.
+
+declare module D: FinRO_Distinguisher{RO, FRO}.
+
+local module GenFinRO (RO:RO) = {
+  include RO [set, rem, get]
+
+  proc init () = {
+    var l;
+    l <- FinFrom.enum;
+    RO.init();
+    while (l <> []) {
+      RO.sample(head witness l);
+      l <- behead l;
+    } 
+  }
+
+  proc sample (x:from) = {
+    RO.get(x);
+  }
+
+}.
+
+local module D' (RO:RO) = MainD (D, GenFinRO(RO)).
+
+local equiv RO_LFinRO_init : RO.init ~ GenFinRO(LRO).init : ={glob RO} ==> ={res, glob RO}.
+proof.
+  proc; inline *.
+  while{2} true (size l{2}); auto; smt (head_behead size_eq0 size_ge0).
+qed.
+
+local equiv GFinRO_RO_init : 
+   GenFinRO(RO).init ~ FinRO.init : 
+     ={RO.m} ==>
+     ={RO.m} /\ forall (x : from), x \in RO.m{1}.
+proof.
+  proc; inline *.
+  while ( ={l, RO.m} /\ (forall x, x \in RO.m \/ x \in l){1}); auto => />;1: smt (head_behead mem_set).
+  by move=> ?; rewrite FinFrom.enumP.
+qed.
+
+equiv RO_FinRO_D : MainD(D,RO).distinguish ~ MainD(D,FinRO).distinguish :
+         ={glob D, RO.m, arg} ==> ={res, glob D}.
+proof.
+  proc *.
+  transitivity*{1} {r <@ MainD(D, GenFinRO(LRO)).distinguish(x); } => //;1:smt().
+  + inline MainD(D, RO).distinguish MainD(D, GenFinRO(LRO)).distinguish; wp.
+    call (_: ={glob RO});2..4: by sim.
+    + by apply RO_LFinRO_init.
+    by call RO_LFinRO_init;wp.
+  transitivity*{1} {r <@ MainD(D,GenFinRO(RO)).distinguish(x); } => //;1:smt().
+  + by symmetry; call (RO_LRO_D D').
+  inline MainD(D, GenFinRO(RO)).distinguish MainD(D, FinRO).distinguish; wp.
+  call (_: ={RO.m} /\ (forall x, x \in RO.m){1}).
+  + by conseq GFinRO_RO_init.
+  + by proc; rcondf{1} ^if; auto => />; 1: smt(); move=> ??; apply sampleto_ll.
+  + by proc; auto; smt(mem_set).
+  + by proc;inline *;rcondf{1} ^if; auto => />; 1: smt(); move=> ??; apply sampleto_ll.
+  by call GFinRO_RO_init; wp.
+qed.
+
+end section PROOFS.
+
+end FinGenEager.
+
